leetcode/longestPrefix.dfy
@@ -1,9 +1,11 @@
 include "../lib/seq.dfy"
+include "../lib/sets.dfy"
 include "../lib/Trie.dfy"
 
 module LongestCommonPrefix {
     import opened Tries
     import opened SeqCustom
+    import opened SetCustom
 
     predicate IsCommonPrefix(prefix: string, strs: set<string>)
     {
@@ -44,28 +46,74 @@ module LongestCommonPrefix {
         ensures forall x :: x in strs ==> x in ToSet(strs)
     {}
 
-    method longestCommonPrefix(strs: seq<string>) returns (prefix: string)
+    twostate lemma AllFreshUnionFresh(ss: set<set<Trie>>)
+        requires forall s :: s in ss ==> forall t :: t in s ==> t.Valid()
+        requires forall s :: s in ss ==> fresh(s)
+        ensures fresh(Union(ss))
+    {
+
+    }
+
+
+
+    // twostate predicate UnionFresh(t: Trie)
+    //     requires t.Valid()
+    //     requires forall k :: k in t.children.Keys ==> fresh(t.children[k].repr)
+    // {
+    //    fresh(Union(set k | k in t.children.Keys :: t.children[k].repr)) 
+    // }
+
+    method {:vcs_split_on_every_assert} longestCommonPrefix(strs: seq<string>) returns (prefix: string)
         requires strs != []
+        requires forall i :: 0 <= i < |strs| ==> strs[i] != ""
         ensures IsCommonPrefix(prefix, ToSet(strs))
         ensures forall prefixes :: prefixes in AllPrefixes(ToSet(strs)) ==> |prefixes| <= |prefix|
     {
         var trie := new Trie();
+        assert fresh(trie.repr);
+        assert trie.Valid();
+        assert fresh(trie);
         label Begin:
         for i := 0 to |strs| 
             invariant allocated(trie)
-            invariant fresh(trie.repr-old@Begin(trie.repr))
+            invariant "" !in strs[0..i]
+            // invariant trie.words != {} ==> trie.children.Keys != {}
+            invariant fresh(trie)
+            invariant fresh(trie.repr)
+            invariant forall k :: k in trie.children.Keys ==> fresh(trie.children[k]) && fresh(trie.children[k].repr)
+            invariant trie.children.Keys == {} ==> fresh(trie.repr)
+            invariant trie.children.Keys != {} ==> fresh(trie.repr)
+            // invariant fresh(Union(set k | k in trie.children.Keys :: trie.children[k].repr)) /// <<EXPLODES!
+            invariant fresh(Union(trie.ReprSet()))
+            // invariant fresh(trie.repr-old@Begin(trie.repr))
             invariant 0 <= i <= |strs|
             invariant trie.Valid()
             invariant trie.words == ToSet(strs[0..i])
-            modifies trie.repr
+            modifies  trie, trie.repr
         {
             assert strs == strs[0..i] + strs[i..];
-            label PreInsert:
+            // label PreInsert:
+            if trie.children.Keys == {} {
+                // assert "" !in trie.words;
+                // assert trie.words == {};
+            } else {
+                UnionHasAll(set k | k in trie.children.Keys :: trie.children[k].repr);
+                NotInAllNotInUnion(set k | k in trie.children.Keys :: trie.children[k].repr, trie);
+                assert trie !in Union(set k | k in trie.children.Keys :: trie.children[k].repr);
+                assert trie.repr == {trie} + Union(set k | k in trie.children.Keys :: trie.children[k].repr);
+                assert Union(set k | k in trie.children.Keys :: trie.children[k].repr) < trie.repr;
+                ghost var foo := set key | key in trie.children.Keys :: trie.children[key].repr;
+                // assert foo == ReprSet(trie);
+
+                // AllFreshUnionFresh(trie.ReprSet());
+                // assert fresh(Union(set k | k in trie.children.Keys :: trie.children[k].repr));
+                // assert trie.words == Union(set k | k in trie.children.Keys :: trie.children[k].repr);
+            }
             trie.insertRecursive(strs[i]);
             assert strs[0..i+1] == strs[0..i] + [strs[i]];
             ToSetConcat(strs[0..i], [strs[i]]);
             ToSetHasAll(strs[0..i+1]);
-            assert trie.words == old@PreInsert(trie.words) + {strs[i]};
+            // assert trie.words == old@PreInsert(trie.words) + {strs[i]};
         }
         assert strs == strs[0..|strs|];
         assert ToSet(strs) == ToSet(strs[0..|strs|]);
@@ -88,7 +136,7 @@ module LongestCommonPrefix {
                 return prefix';
             }
         }
-        return "";
+        return prefix;
     }
 
 }
